theories/interop/lang_to_mlang.v
@@ -12,11 +12,11 @@ Section ToMlang.
   Local Notation expr_state := ((Λ.(expr) * Λ.(state)))%type.
 
   Inductive prim_step_mrel : prog -> expr_state -> (expr_state->Prop) -> Prop := 
-  | WrapStep p e1 σ1 e2 σ2 (X : _ → Prop) : 
+  | LiftStep p e1 σ1 e2 σ2 (X : _ → Prop) : 
         prim_step p e1 σ1 e2 σ2 [] → 
         (X (e2, σ2)) →
       prim_step_mrel p (e1,σ1) X
-  | WrapUbStep p e1 σ1 X :
+  | LiftUbStep p e1 σ1 X :
         stuck_no_threads p e1 σ1 →
       prim_step_mrel p (e1,σ1) X.
 
@@ -24,8 +24,8 @@ Section ToMlang.
     {| mrel := prim_step_mrel p |}.
   Next Obligation.
     intros p. intros [e1 σ1] X Y Hstep HXY. inversion Hstep; subst.
-    - eapply (WrapStep p e1 σ1 e2 σ2); first done. apply HXY, H4.
-    - by eapply (WrapUbStep p e1 σ1).
+    - eapply (LiftStep p e1 σ1 e2 σ2); first done. apply HXY, H4.
+    - by eapply (LiftUbStep p e1 σ1).
   Qed.
 
   Notation cont := Λ.(ectx).
@@ -48,20 +48,20 @@ Section ToMlang.
       + inversion H; simplify_eq.
         * apply prim_step_call_inv in H3 as (er&fn&HH1&HH2&->&->&_).
           intros ? ? ? ?; simplify_eq; simplify_map_eq; congruence.
-        * destruct H4 as [Hv Hpr]. intros fn e2 HH1 HH2; exfalso; eapply Hpr. 1: exact nil.
+        * destruct H4 as [Hv Hpr]. intros fn e2 HH1 HH2; exfalso; eapply Hpr.
           eapply fill_prim_step, head_prim_step, call_head_step. by repeat eexists.
       + destruct (p !! f) as [fn|] eqn:Heq1; first destruct (apply_func fn vs) as [e2|] eqn:Heq2.
-        * eapply WrapStep; last by eapply H.
+        * eapply LiftStep; last by eapply H.
           eapply fill_prim_step, head_prim_step, call_head_step. by repeat eexists.
-        * eapply WrapUbStep. split; first apply to_val_fill_call.
-          intros e' σ' efs (er&fn'&HH1&HH2&->&->&_)%prim_step_call_inv; repeat simplify_eq. congruence.
-        * eapply WrapUbStep. split; first apply to_val_fill_call.
-          intros e' σ' efs (er&fn'&HH1&HH2&->&->&_)%prim_step_call_inv; repeat simplify_eq.
+        * eapply LiftUbStep. split; first apply to_val_fill_call.
+          intros e' σ' (er&fn'&HH1&HH2&->&->&_)%prim_step_call_inv; repeat simplify_eq. congruence.
+        * eapply LiftUbStep. split; first apply to_val_fill_call.
+          intros e' σ' (er&fn'&HH1&HH2&->&->&_)%prim_step_call_inv; repeat simplify_eq.
     - intros e [v Hv] f vs C ->. rewrite to_val_fill_call in Hv; done.
     - intros p e σ H.
       destruct (XM (∃ e2 σ2, language.prim_step p e σ e2 σ2 [])) as [(e2&σ2&Hl)|Hr].
-      + eapply WrapStep; last done. exact Hl.
-      + eapply WrapUbStep. split; first done. intros ? ? ? ?. eapply Hr. by do 2 eexists.
+      + eapply LiftStep; last done. exact Hl.
+      + eapply LiftUbStep. split; first done. intros ? ? ?. eapply Hr. by do 2 eexists.
   Qed.
 
   Definition lang_to_mlang : mlanguage val :=
