theories/interop/lang_to_mlang_wp.v
@@ -4,7 +4,7 @@ From melocoton.interop Require Import lang_to_mlang.
 From melocoton.mlanguage Require Import mlanguage.
 From melocoton.language Require Import language weakestpre.
 From melocoton.mlanguage Require Import weakestpre.
-From melocoton.interop Require Import linking_wp.
+(* From melocoton.interop Require Import linking_wp. *)
 From iris.proofmode Require Import proofmode.
 
 Section ToMlang_logic.
@@ -25,22 +25,26 @@ Global Program Instance lang_to_mlang_mlangGS :
   at_boundary := True%I;
 }.
 
+(*
+
 Global Program Instance lang_to_mlang_linkableGS :
   (@linkableGS _ _ (lang_to_mlang Λ) _ _ (lang_to_mlang_linkable Λ) state_interp)%I
 := {
   private_state_interp := (λ _, True)%I;
-}.
+}. 
 Next Obligation. simpl. intros *. inversion 1. iIntros "?". by iFrame. Qed.
 Next Obligation.
   simpl. intros ? []. iIntros "? _". iModIntro. iExists _. by iFrame.
 Qed.
 Next Obligation. simpl. iIntros (σ) "_ Hσ". iPureIntro. exists σ, (). constructor. Qed.
-
+*)
 (* This is a *local* instance to allow typechecking the lemma below. The idea is
    that it should stay local. For each specific language, one should manually
    define the corresponding mlanguage (by applying lang_to_mlang), and define it
    there as a canonical structure. *)
 Local Canonical Structure lang_to_mlang_mlang : mlanguage val := lang_to_mlang Λ.
+
+Notation mkPE p T := (@Build_prog_environ _ _ _ p T).
 
 Definition penv_to_mlang (pe : language.weakestpre.prog_environ Λ Σ) :
   mlanguage.weakestpre.prog_environ (lang_to_mlang Λ) Σ
@@ -54,18 +58,89 @@ Proof using.
   iStartProof. iLöb as "IH" forall (e). destruct pe as [p T].
   rewrite {1} @language.weakestpre.wp_unfold /language.weakestpre.wp_pre. simpl.
   rewrite {1} wp_unfold /mlanguage.weakestpre.wp_pre.
-  iIntros "H" (σ) "(%n & Hσ)". iMod ("H" $! σ n with "Hσ") as "[(%x & %H1 & Hσ & H)|[(%s' & %vv & %K' & %H1 & %H2 & H3)|(%Hred & H3)]]".
+  iIntros "H" (σ) "(%n & Hσ)". iMod ("H" $! σ n with "Hσ") as "[(%x & %H1 & Hσ & H)|[(%s' & %vv & %K' & %H1 & %H2 & H3)|(%Hred & H3)]]"; cbn.
   - iLeft. iModIntro. iExists x. iFrame. iSplitR; first done. iExists n. iFrame.
   - iRight. iLeft. iMod "H3" as "(%Ξ & Hσ & HT & Hr)". iExists s', vv, K'. iModIntro.
     iSplitR; first done. iSplitR; first done. iSplitR; first done. iSplitL "Hσ"; first by iExists n.
     iExists Ξ. iFrame. iNext. iIntros (v) "[Hv _]". iApply "IH". by iApply "Hr".
   - iRight. iRight. iModIntro. iSplitR.
-    { iPureIntro. destruct Hred as (e' & σ' & H'). eexists (fun '(e2,σ2) => e2 = e' ∧ σ2 = σ'). inversion H'; subst. econstructor. eexists; split; first done.
-      econstructor; first done. intros ? ? ( <- & <- ); done. }
-    iIntros (X Hstep). inversion Hstep as (K & e' & -> & Hx). inversion Hx; subst.
-    unshelve iMod ("H3" $! σ2 _ (Prim_step _ K _ _ _ _ _ _ _ _ _ H3)) as "H3". 1-2:done.
-    do 2 iModIntro. iMod "H3" as "(Hσ & Hwp)". iModIntro. iExists _, _. iSplitR; first (iPureIntro; apply H5; repeat split).
-    iSplitL "Hσ"; first by iExists _. iApply "IH". iApply "Hwp".
+    { iPureIntro. eapply reducible_not_val. destruct Hred as (?&?&?); by do 3 eexists. }
+    iIntros (X Hstep). inversion Hstep; simplify_eq.
+    + iMod ("H3" $! σ2 e2 H3) as "H3". do 2 iModIntro. iMod "H3" as "(Hσ&HWP)". iModIntro. 
+      do 2 iExists _; iSplit; first done.
+      iSplitL "Hσ"; first by iExists _.
+      iApply "IH". done.
+    + destruct H4 as [_ H4%not_reducible_no_threads]. exfalso; tauto.
+Qed.
+
+Lemma wp_lang_to_mlang_backwards (e : Λ.(language.expr)) pe E Φ :
+  ⊢ WP e @ (penv_to_mlang pe); E {{ Φ }} -∗ WP e @ pe; E {{ Φ }}.
+Proof using.
+  iStartProof. iLöb as "IH" forall (e). destruct pe as [p T].
+  rewrite {1} @language.weakestpre.wp_unfold /language.weakestpre.wp_pre. simpl.
+  rewrite {1} wp_unfold /mlanguage.weakestpre.wp_pre.
+  iIntros "H" (σ n) "Hσ".
+  iMod ("H" $! σ with "[Hσ]") as "[(%x & %H1 & Hσ & H)|[(%s' & %vv & %K' & %Hcall & %H2 & _ & (%n0 & Hσ) & H3)|(%Hred & H3)]]"; cbn.
+  - iExists n; done.
+  - iLeft. iModIntro. iExists x. iFrame. iSplitR; first done. iDestruct "Hσ" as "(%&HH)".
+    assert (n = n0) as -> by admit. done.
+  - iRight. iLeft. cbn in Hcall. unfold lang_to_mlang.is_call in Hcall. subst e.
+    iModIntro. do 3 iExists _; iSplit; first done.
+    iSplit; first done.
+    iPoseProof "H3" as "(%Ξ & HT & Hr)". iModIntro. iExists Ξ.
+    assert (n = n0) as -> by admit. iFrame.
+    iNext. iIntros (v) "Hv". iApply "IH". iApply "Hr". iFrame.
+  - iRight. iRight. iModIntro.
+    eapply (prim_step_is_total p e σ) in Hred as Hstep.
+    inversion Hstep; simplify_eq.
+    2: { iPoseProof ("H3" $! (λ _, False) (LiftUbStep _ p e σ _ H4)) as "H3".
+         iAssert (|={E}▷=> False)%I with "[H3]" as "Halmost_false".
+         1: iMod "H3"; do 2 iModIntro; iMod "H3" as "(%&%&[]&_)".
+         Fail iApply "Halmost_false". admit. }
+    iSplit.
+    1: iPureIntro; by do 2 eexists.
+    iIntros (σ3 e3 Hstep2).
+    assert (prim_step p (e, σ) (λ '(e4,σ4), e4=e3 ∧ σ4=σ3)) as HstepW.
+    1: eapply LiftStep; done.
+    iMod ("H3" $! _ HstepW) as "H3". do 2 iModIntro.
+    iMod "H3" as "(%e4&%σ4&(->&->)&(%n0&Hσ)&HWP)". iModIntro.
+    assert (S n = n0) as -> by admit. iFrame.
+    iApply "IH". done.
+Abort.
+
+
+Lemma wp_lang_to_mlang_bind K pe E e Φ :
+  WP e @ (penv_to_mlang pe); E {{ v, WP fill K (of_class _ (ExprVal v)) @ (penv_to_mlang pe); E {{ Φ }} }} ⊢ WP fill K e @ (penv_to_mlang pe); E {{ Φ }}.
+Proof.
+  iIntros "H". iLöb as "IH" forall (E e Φ). rewrite !wp_unfold /wp_pre.
+  iIntros "%σ Hσ".
+  iMod ("H" $! σ with "Hσ") as "[(%x & -> & Hσ & H)|[(%s & %vv & %K' & %HH & %H2 & Hb & Hσ & %Ξ & HT & Hr)|(%Hnv&H3)]]".
+  - rewrite {1} wp_unfold /wp_pre.
+    iMod ("H" $! σ with "Hσ") as "H". iModIntro. iApply "H".
+  - iModIntro. iRight. iLeft. iExists s, vv, (comp_ectx K K').
+    rewrite /is_call /= /lang_to_mlang.is_call in HH; subst e.
+    iSplitR; first by erewrite (fill_comp K K').
+    iSplitR; first done. iFrame.
+    iExists Ξ. iFrame. iNext.
+    iIntros "%r HΞ". rewrite /resume_with /=.
+    rewrite <- fill_comp.
+    iApply "IH". iApply ("Hr" with "HΞ").
+  - iRight. iRight. iModIntro. iSplit. 
+    1: iPureIntro; by apply fill_not_val.
+    iIntros (X Hstep). inversion Hstep; simplify_eq.
+    + eapply fill_step_inv in H3 as (e2'&->&Hstep'); last done.
+      assert (prim_step (penv_prog (penv_to_mlang pe)) (e, σ) (λ '(e4,σ4), e4=e2' ∧ σ4=σ2)) as HstepW.
+      1: eapply LiftStep; done.
+      iMod ("H3" $! _ HstepW) as "H3". do 2 iModIntro.
+      iMod "H3" as "(%e4&%σ4&(->&->)&(%n0&Hσ)&HWP)". iModIntro.
+      do 2 iExists _. iSplit; first done.
+      iSplitL "Hσ"; first by iExists _. iApply "IH". done.
+    + destruct H4 as [Hnvf Hst].
+      assert (stuck_no_threads (penv_prog (penv_to_mlang pe)) e σ) as Hirred.
+      { split; first done. intros ? ? ?. eapply (Hst (fill K e') σ').
+        eapply fill_prim_step. done. }
+      iMod ("H3" $! (λ _, False) (LiftUbStep _ _ _ _ _ Hirred)) as "H3".
+      do 2 iModIntro. iMod "H3" as "(%&%&[]&_)".
 Qed.
 
 End ToMlang_logic.
